geach

Foundation/Semantics/Kripke/Basic.lean
@@ -11,37 +11,104 @@ variable {α : Type u}
 structure KripkeFrame (α : Type u) where
   points : Set α
   points_nonempty : points.Nonempty
-  Rel : α → α → Prop
+  rel : α → α → Prop
 
 namespace KripkeFrame
 
 variable {K : KripkeFrame α}
 
+abbrev restrictedRel {K : KripkeFrame α} (x y : K.points) := K.rel x y
+infix:50 " ≺ " => restrictedRel
+
+
 class Generated (K : KripkeFrame α) (R : Set K.points) (hR : R ≠ ∅) : Prop where
-  generated : ∀ x : K.points, ∃ r ∈ R, K.Rel r x
+  generated : ∀ x, ∃ r ∈ R, r ≺ x
 alias generated := Generated.generated
 
 
 class Rooted (K : KripkeFrame α) (r : K.points) extends Generated K {r} (by simp)
 @[grind .]
-lemma rooted {r} [hR : K.Rooted r] : ∀ x : K.points, K.Rel r x := by simpa using hR.generated;
+lemma rooted {r} [hR : K.Rooted r] : ∀ x : K.points, r ≺ x := by simpa using hR.generated;
 
 
-
-class Reflexive (K : KripkeFrame α) extends Std.Refl (α := K.points) (K.Rel ↑· ↑·)
+class Reflexive (K : KripkeFrame α) extends Std.Refl (α := K.points) (· ≺ ·)
 @[grind .]
-lemma refl [hRefl : K.Reflexive] : ∀ x : K.points, K.Rel ↑x ↑x := hRefl.refl
+lemma refl [hRefl : K.Reflexive] : ∀ x : K.points, x ≺ x := hRefl.refl
 
 
-class Transitive (K : KripkeFrame α) extends IsTrans (α := K.points) (K.Rel ↑· ↑·)
+class Transitive (K : KripkeFrame α) extends IsTrans (α := K.points) (· ≺ ·)
 @[trans]
-lemma trans [hTrans : K.Transitive] : ∀ x y z : K.points, K.Rel ↑x ↑y → K.Rel ↑y ↑z → K.Rel ↑x ↑z := hTrans.trans
+lemma trans [hTrans : K.Transitive] : ∀ x y z : K.points, x ≺ y → y ≺ z → x ≺ z := hTrans.trans
 
 
-class Preorder (K : KripkeFrame α) extends IsPreorder (α := K.points) (K.Rel ↑· ↑·)
+class Preorder (K : KripkeFrame α) extends IsPreorder (α := K.points) (· ≺ ·)
+instance [K.Preorder] : K.Reflexive where
+instance [K.Preorder] : K.Transitive where
+
+section Iterate
+
+variable {K : KripkeFrame α}
+variable {x y : K.points}
+variable {n m : ℕ}
+
+def restrictedRelI {K : KripkeFrame α} : ℕ → Rel K.points K.points
+  | 0 => (· = ·)
+  | n + 1 => fun x y ↦ ∃ z, x ≺ z ∧ K.restrictedRelI n z y
+notation x:80 " ≺^[" n "] " y:80 => restrictedRelI n x y
+
+@[simp, grind .] lemma relI_zero : x ≺^[0] y ↔ (x = y) := by tauto;
+@[simp, grind .] lemma relI_one : x ≺^[1] y ↔ x ≺ y := by simp [restrictedRelI];
+lemma relI_succ_right : x ≺^[n + 1] y ↔ (∃ z, x ≺ z ∧ z ≺^[n] y) := by tauto;
+
+lemma relI_comp : x ≺^[n + m] y ↔ ∃ z, x ≺^[n] z ∧ z ≺^[m] y := by
+  induction n generalizing x y with
+  | zero => grind;
+  | succ n ih =>
+    suffices x ≺^[(n + m) + 1] y ↔ ∃ z, x ≺^[(n + 1)] z ∧ z ≺^[m] y by grind;
+    constructor;
+    . rintro ⟨w, Rxw, Rwy⟩;
+      obtain ⟨z, Rwz, Rzy⟩ := ih.mp Rwy;
+      use z;
+      constructor;
+      . use w;
+      . assumption;
+    . rintro ⟨z, ⟨w, Rxw, Rwz⟩, Rzy⟩;
+      use w;
+      constructor;
+      . assumption;
+      . apply ih.mpr;
+        use z;
+
+lemma relI_succ_left : x ≺^[n + 1] y ↔ ∃ z, x ≺^[n] z ∧ z ≺ y := by simpa using relI_comp (n := n) (m := 1);
+
+@[grind →]
+lemma unwrap_of_trans [K.Transitive] {n : ℕ+} (Rxy : x ≺^[n] y) : x ≺ y := by
+  induction n using PNat.recOn generalizing x with
+  | one => simpa using Rxy;
+  | succ n ih =>
+    obtain ⟨z, Rxz, Rzy⟩ := Rxy;
+    exact K.trans x z y Rxz $ ih Rzy;
+
+@[grind →]
+lemma unwrap_of_trans' [K.Transitive] {n : ℕ} (hn : 0 < n) (Rxy : x ≺^[n] y) : x ≺ y :=
+  unwrap_of_trans (n := ⟨n, by omega⟩) Rxy
+
+@[grind →]
+lemma unwrap_of_preorder [K.Preorder] {n : ℕ} (Rxy : x ≺^[n] y) : x ≺ y := by
+  induction n with
+  | zero =>
+    subst Rxy;
+    apply K.refl;
+  | succ n ih =>
+    exact unwrap_of_trans' (by omega) Rxy;
+
+end Iterate
+
 
 
 end KripkeFrame
+
+
 
 end LO
 
